pulse/tests/micro-benchmarks/SteelIntroExists.fst
@@ -1,0 +1,283 @@
+(*
+
+Experimenting with automating the introduction of existentials
+
+
+1. Difficulties in applying intro_exists:
+
+ {  A  }
+
+    { ?p ?w }
+     intro_exists ?w ?p
+    { ex ?p }
+
+ { ex ?p * ?f }
+
+ { ... }
+
+This requires solving, since intro_exists is framed:
+
+  A =?=> ?p ?w * ?f
+
+This can't be solved since we have two unknowns on the LHS.
+
+--------------------------------------------------------------------------------
+2.
+
+One might consider turning intro_exists into the SteelF effect, so
+that we don't add another frame, but that's not what's desired either.
+
+Consider:
+
+  val free (p:ptr) : ST _ (ex (fun v -> p `pts_to` v)) emp
+
+
+let caller (p q:ptr) : ST _ (p `pts_to` 17 `star` q `pts_to` 18) =
+  intro_exists _ _; //if this were not framed
+                    //then we would capture both p and q under the exists
+                    //and this wouldn't unify with the pre of `free p` anyway
+  free p
+
+--------------------------------------------------------------------------------
+
+So, our idea is to enhance the framing tactic directly so that it can
+introduce existentials "on the fly" without introducing additional
+vprop variables, as in case 1.
+
+i.e. we want to write
+
+
+let caller (p q:ptr) : ST _ (p `pts_to` 17 `star` q `pts_to` 18) =
+  free p;
+  ...
+
+And this would generate constraints like so
+
+{  p `pts_to` 17 `star` q `pts_to` 18 }
+
+    { ex (pts_to p) }
+      free p
+    { emp }
+
+{emp * ?f }
+
+
+and we would try to solve
+
+
+p `pts_to` 17 `star` q `pts_to` 18
+==>
+ex (pts_to p) * ?f
+
+And this has only 1 unknown, so we have some hope of solving for ?f
+
+The basic idea is as follows:
+
+In case the current unification heuristics fail, i.e.,
+
+  1. let LEX = { ex p1, .., ex pn } be all the unique occurrences of
+     ex terms on the LHS
+
+  2. let REX = { ex q1, .., ex qm } be all the unique occurrences of
+     ex terms on the RLHS
+
+  3. Cancel terms in LEX with terms from REX:
+
+     For each element l in LEX, find a unique element r in REX such
+     that l unifies with r.
+
+       - If successful, remove l and r from LEX and REX and repeat
+
+       - If not, fail: there is an exists in LEX that cannot be
+         matched in REX.
+
+     Limitation: We are not handling AC rewriting under a quantifier, e.g.,
+
+        ex (fun v -> p * q)  will not match
+        ex (fun v -> q * p)
+
+     We could enhance this step, so that rather than finding a unifier
+     between l and r, we find instead a double implication, e.g., by
+     applying lemma like equiv_exists
+
+     Lemma (forall v. p v <==> q v)
+           (ex p <==> ex q)
+
+
+  4. Now, we may have some remaining terms in REX and for these we aim
+     to introduce exists from the remaining terms in L
+
+
+     1. For each r in REX, open the existential with a fresh
+          unification variable for the witness
+
+        This corresponds to an application of the following logical rule
+       "backwards" to the goal:
+
+       intro_exists (x:a) (v: a -> vprop)
+          : Lemma (v x `can_be_split` (ex v))
+
+     2. unifying what's left in RHS with whatever was not yet cancelled in LHS
+*)
+module SteelIntroExists
+open Steel.Effect.Common
+open Steel.ST.Util
+
+module T = FStar.Tactics
+
+#set-options "--ide_id_info_off"
+
+assume
+val ptr : Type0
+
+assume
+val pts_to (p:ptr) (v:nat) : vprop
+
+assume
+val free (p:ptr) : STT unit (exists_ (fun v -> pts_to p v)) (fun _ -> emp)
+
+let free_one_default (p q r:ptr)
+  : STT unit
+    (pts_to p 17 `star` pts_to q 18 `star` pts_to r 19)
+    (fun _ -> pts_to p 17 `star` pts_to r 19)
+ = intro_exists _ (fun v -> pts_to q v);
+   let _ = free q in ()
+
+// assume
+// val intro_exists_f (#a:Type) (#opened_invariants:_) (x:a) (p:a -> vprop)
+//   : STGhostF unit opened_invariants (p x) (fun _ -> exists_ (fun v -> p v)) (True) (fun _ -> True)
+
+
+// // [@@expect_failure] //we incorrectly pick a too-specific solution failing to generalize over the witness
+// // let free_one_explicit (p q:ptr)
+// //   : STT unit
+// //     (pts_to p 17)
+// //     (fun _ -> emp)
+// //  = let _ = intro_exists_f 17 _  in
+// //    free p
+// //#push-options "--tactic_trace_d 1"
+
+let free_one (p q r:ptr)
+  : STT unit
+    (pts_to p 17 `star` pts_to q 18 `star` pts_to r 19)
+    (fun _ -> pts_to p 17 `star` pts_to r 19)
+ = let _ = free q in ()
+
+assume
+val free2 (p q:ptr) : STT unit (exists_ (fun v -> pts_to p v) `star`
+                                exists_ (fun v -> pts_to q v))
+                               (fun _ -> emp)
+
+
+let free_two (p q r:ptr)
+  : STT unit
+    (pts_to p 17 `star` pts_to q 18 `star` pts_to r 19)
+    (fun _ -> pts_to r 19)
+ = free p; free q; ()
+
+assume
+val correlate (p q:ptr) : STT unit (exists_ (fun v -> pts_to p v `star` pts_to q v))
+                                   (fun _ -> emp)
+
+let free_correlate (p q:ptr)
+  : STT unit
+    (pts_to q 17 `star` pts_to p 17)
+    (fun _ -> emp)
+ = correlate p q; ()
+
+
+let free_correlate_alt (p q:ptr)
+  : STT unit
+    (pts_to p 17 `star` pts_to q 17)
+    (fun _ -> emp)
+ = correlate p q; ()
+
+assume
+val alloc (n:nat) : STT ptr emp (fun p -> pts_to p n)
+
+let construct () : STT ptr emp (fun p -> exists_ (fun v -> pts_to p v)) =
+  let p = alloc 17 in
+  p
+
+assume
+val write (p: ptr) (n: nat) : STT unit (exists_ (fun n' -> pts_to p n')) (fun _ -> pts_to p n)
+
+assume
+val pts_to_rev (n:nat) (p:ptr) : vprop
+
+assume
+val alloc_rev (n:nat) : STT ptr emp (fun p -> pts_to_rev n p)
+
+
+let construct_rev () : STT ptr emp (fun p -> exists_ (fun v -> pts_to_rev v p)) =
+  let p = alloc_rev 17 in
+  p
+
+let test_exists_intro_pure
+  (p: ptr)
+: STT unit (exists_ (fun n -> pts_to p n)) (fun _ -> exists_ (fun n -> pts_to p n `star` pure (n == 18)))
+=
+  write p 18;
+  ()
+
+let test_exists_intro_pure2
+  (p: ptr)
+: STT unit (exists_ (fun n -> pts_to p n)) (fun _ -> exists_ (fun n -> pts_to p n `star` pure (n == 18)))
+=
+  write p 42;
+  write p 18;
+  ()
+
+let test_exists_intro_pure'
+  (p: ptr)
+  (i:nat)
+: STT unit (exists_ (fun n -> pts_to p n)) (fun _ -> exists_ (fun n -> pts_to p n `star` pure (n == 18)))
+= if i = 18
+  then
+    let h : squash (i == 18) = () in
+    let _ = write p i in
+    ()
+  else let _ = write p 18 in ()
+
+let test_exists_intro_pure''
+  (p: ptr)
+  (i:nat)
+: STT unit (exists_ (fun n -> pts_to p n)) (fun _ -> exists_ (fun n -> pts_to p n `star` pure (n == 18)))
+= if i = 18
+  then
+    let _ = write p i in
+    ()
+  else let _ = write p 18 in ()
+
+let test_intro_pure
+  (x: int)
+  (sq: squash (x == 18))
+: STT unit emp (fun _ -> pure (x == 18))
+= 
+  let _ = () in
+  return ()
+
+let test_intro_pure'
+  (x: int)
+: ST unit emp (fun _ -> pure (x == 18)) (requires (x == 18)) (ensures (fun _ -> True))
+= 
+  let _ = noop () in
+  return ()
+
+assume val decr_weak
+  (p: ptr)
+: STT unit (exists_ (fun x -> p `pts_to` x `star` pure (if x > 0 then True else False))) (fun _ -> exists_ (fun x -> p `pts_to` x))
+
+let test_decr_weak
+  (p: ptr)
+: STT unit (exists_ (fun x -> p `pts_to` x)) (fun _ -> exists_ (fun x -> p `pts_to` x))
+= write p 42; // good news: replacing with 0 will correctly make the error message point to the violated precondition in decr_weak
+  decr_weak p;
+  return ()
+
+assume
+val pred ([@@@smt_fallback] _ : nat) : vprop
+
+let test (x y:nat) : ST unit (pred x) (fun _ -> pred 17 `star` pure ((x > y)==true)) (requires x == 17 /\ x > y) (ensures fun _ -> True) =
+ let _ = noop () in 
+ return ()
